src/IsoCan.v
@@ -1,4 +1,4 @@
-From mathcomp Require Import all_ssreflect fingraph.
+From mathcomp Require Import all_ssreflect.
 Set Implicit Arguments.
 Unset Strict Implicit.
 Unset Printing Implicit Defensive.
